DEX_StaticHandler.v
@@ -1,0 +1,185 @@
+(** * Bicolano: StaticHandler for exceptions *)
+
+Require Export DEX_BigStep.
+
+Module DEX_StaticHandler.
+  
+  Import DEX_BigStep.DEX_Dom.DEX_Prog.
+
+  Section DEX_subclass_test.
+    Variable p : DEX_Program.
+    Variable DEX_subclass_test : DEX_ClassName -> DEX_ClassName -> bool.
+    Variable DEX_subclass_test_correct :
+      forall c1 c2,
+        if DEX_subclass_test c1 c2 then subclass_name p c1 c2
+          else ~ subclass_name p c1 c2.
+
+(*    Fixpoint search_handler (pc:PC) (c:ClassName)
+      (l:list ExceptionHandler) {struct l} : option ExceptionHandler :=
+      match l with
+        nil => None
+        | h::q => 
+          match EXCEPTIONHANDLER.catchType h with
+            None => 
+            (if EXCEPTIONHANDLER.isPCinRange h pc then Some h
+              else search_handler pc c q)
+            | Some ch => 
+              if subclass_test c ch then
+                (if EXCEPTIONHANDLER.isPCinRange h pc then Some h
+                  else search_handler pc c q)
+                else search_handler pc c q
+          end
+      end.
+
+    Definition handler (m:Method) (pc:PC) (cl:ClassName) : option PC :=
+      match METHOD.body m with
+        None => None
+        | Some bm =>
+          match search_handler pc cl (BYTECODEMETHOD.exceptionHandlers bm) with
+            None => None
+            | Some h => Some (EXCEPTIONHANDLER.handler h)
+          end
+      end.
+
+    Ltac caseeq t := generalize (refl_equal t); pattern t at -1 in |- * ; case t.
+
+    Lemma lookup_handlers_search_handler : forall hs pc pc' cn,
+      lookup_handlers p hs pc cn pc' ->
+      exists hd, search_handler pc cn hs = Some hd
+        /\ pc' = EXCEPTIONHANDLER.handler hd.
+    Proof.
+      induction hs; intros.
+      inversion_clear H.
+      inversion_clear H; simpl.
+      exists a; split; auto.
+      inversion_clear H0.
+      rewrite H.
+      rewrite H1.
+      auto.
+      rewrite H.
+      generalize (subclass_test_correct cn cl1).
+      destruct (subclass_test cn cl1); intros; try (intuition;fail).
+      rewrite H1; auto.
+      destruct (IHhs _ _ _ H1) as [hd [HH1 HH2]].
+      caseeq (EXCEPTIONHANDLER.catchType a); intros.
+      generalize (subclass_test_correct cn c).
+      destruct (subclass_test cn c); intros; try (intuition;fail).
+      caseeq (EXCEPTIONHANDLER.isPCinRange a pc); intros.
+      elim H0; constructor 2 with c; auto.
+      exists hd; auto.
+      exists hd; auto.
+      caseeq (EXCEPTIONHANDLER.isPCinRange a pc); intros.
+      elim H0; constructor 1; auto.
+      auto.
+    Qed.
+
+    Lemma search_handler_lookup_handlers : forall hs pc cn hd,
+      search_handler pc cn hs = Some hd ->
+      lookup_handlers p hs pc cn (EXCEPTIONHANDLER.handler hd).
+    Proof.
+      induction hs; simpl; intros.
+      discriminate.
+      generalize H; clear H.
+      caseeq (EXCEPTIONHANDLER.catchType a); [intros c Hc|intros Hc].
+      generalize (subclass_test_correct cn c).
+      destruct (subclass_test cn c).
+      caseeq (EXCEPTIONHANDLER.isPCinRange a pc); intros.
+      injection H1; clear H1; intros; subst.
+      constructor 1.
+      constructor 2 with c; auto.
+      constructor 2; eauto.
+      intro.
+      inversion_clear H2.
+      rewrite Hc in H3; discriminate.
+      rewrite H in H4; discriminate.
+      intros; constructor 2; eauto.
+      intro.
+      inversion_clear H1.
+      rewrite Hc in H2; discriminate.
+      rewrite Hc in H2; injection H2; intros; subst.
+      contradiction.
+      caseeq (EXCEPTIONHANDLER.isPCinRange a pc); intros.
+      injection H0; clear H0; intros; subst.
+      constructor 1.
+      constructor 1; auto.
+      constructor 2; eauto.
+      intro.
+      inversion_clear H1.
+      rewrite H in H3; discriminate.
+      rewrite H in H3; discriminate.
+    Qed.
+*)
+  End DEX_subclass_test.
+
+End DEX_StaticHandler.
+
+Module DEX_StaticHandlerProp.
+
+  Import DEX_StaticHandler DEX_BigStep.DEX_BigStep DEX_Dom DEX_Prog.
+  
+  Section DEX_subclass_test.
+    Variable p : DEX_Program.
+    Variable DEX_subclass_test : DEX_ClassName -> DEX_ClassName -> bool.
+    Variable DEX_subclass_test_correct :
+      forall c1 c2,
+        if DEX_subclass_test c1 c2 then subclass_name p c1 c2
+          else ~ subclass_name p c1 c2.
+(*
+    Lemma CaughtException_handler :
+      forall m pc h loc pc' cn,
+        Heap.typeof h loc = Some (Heap.LocationObject cn) ->
+        CaughtException p m (pc,h,loc) pc' ->
+        handler subclass_test m pc cn = Some pc'.
+    Proof.
+      intros.
+      inversion_clear H0.
+      elim (lookup_handlers_search_handler p _ subclass_test_correct)
+        with (1:=H3); intros hd [HH1 HH2].
+      unfold handler.
+      rewrite H1.
+      rewrite H2 in H; inversion H; subst.
+      rewrite HH1; auto.  
+    Qed.
+
+    Lemma handler_CaughtException :
+      forall m pc h loc pc' cn,
+        Heap.typeof h loc = Some (Heap.LocationObject cn) ->
+        handler subclass_test m pc cn = Some pc' ->
+        CaughtException p m (pc,h,loc) pc'.
+    Proof.
+      intros until 1.
+      unfold handler.
+      case_eq (METHOD.body m); [intros bm Hbm|intros Hbm].
+      case_eq (search_handler subclass_test pc cn (BYTECODEMETHOD.exceptionHandlers bm)); intros; try discriminate.
+      constructor 1 with bm cn; auto.
+      injection H1; clear H1; intros; subst.
+      apply (search_handler_lookup_handlers p _ subclass_test_correct); auto.
+      intros; discriminate.
+    Qed.
+
+    Lemma no_handler_no_CaughtException :
+      forall m pc h loc cn,
+        Heap.typeof h loc = Some (Heap.LocationObject cn) ->
+        handler subclass_test m pc cn = None ->
+        forall pc', ~ CaughtException p m (pc,h,loc) pc'.
+    Proof.
+      red; intros.
+      rewrite (CaughtException_handler m pc h loc pc' cn H H1) in H0; discriminate.
+    Qed.
+
+    Lemma no_CaughtException_no_handler :
+      forall m pc h loc cn,
+        Heap.typeof h loc = Some (Heap.LocationObject cn) ->
+        (forall pc', ~ CaughtException p m (pc,h,loc) pc') ->
+        handler subclass_test m pc cn = None.
+    Proof.
+      intros.
+      case_eq (handler subclass_test m pc cn); intros; auto.
+      elim (H0 p0).
+      eapply handler_CaughtException; eauto.
+    Qed. 
+*)
+  End DEX_subclass_test.
+
+End DEX_StaticHandlerProp.
+
