DEX_typing_rules.v
@@ -1,0 +1,874 @@
+(** typing_rules.v: Typing rules, plus an executable type checker *)
+Require Export DEX_BigStepAnnot.
+Require Export Bool.
+Require Export DEX_step.
+Import DEX_StaticHandler.DEX_StaticHandler DEX_BigStep.DEX_BigStep DEX_Dom.DEX_Prog.
+
+Import Level.L.
+Import DEX_Dom.
+
+Open Scope type_scope.
+
+  Section DEX_typing_rules.   (** Typing rules **)
+    Variable p : DEX_ExtendedProgram.
+    Variable subclass_test : DEX_ClassName -> DEX_ClassName -> bool.
+    Variable subclass_test_correct :
+      forall c1 c2,
+        if subclass_test c1 c2 then subclass_name p.(DEX_prog) c1 c2
+          else ~ subclass_name p.(DEX_prog) c1 c2.
+    Variable m : DEX_Method.
+    Definition method_signature := DEX_METHOD.signature m.
+    Variable sgn : DEX_sign.
+    Variable region : DEX_PC -> DEX_tag -> DEX_PC -> Prop.
+    Variable se : DEX_PC -> L.t.
+    Variable selift : DEX_PC -> DEX_tag -> L.t -> bool.
+
+    (* Notation handler := (handler subclass_test m). *)
+
+    Infix "<=" := L.leql (at level 70).
+    Infix "<='" := L.leql' (at level 70).
+    Infix "U'" := L.join' (at level 60, right associativity).
+    Infix "U" := L.join (at level 60, right associativity).
+
+    Inductive texec : DEX_PC -> DEX_Instruction -> DEX_tag -> TypeRegisters -> option TypeRegisters -> Prop :=
+    | nop : forall i rt,
+      texec i Nop None rt (Some rt)
+
+    | move_constrained : forall i (rt:TypeRegisters) k_rs (k:DEX_ValKind) (r:DEX_Reg) (rs:DEX_Reg),
+      In r (locR p method_signature) ->
+      Some k_rs = BinNatMap.get _ rt rs ->
+      se i <= sgn.(DEX_lvt) r ->
+      k_rs <= sgn.(DEX_lvt) r ->
+      texec i (Move k r rs) None rt 
+       (Some (BinNatMap.update _ rt r ((se i) U' k_rs)))
+
+    | move_unconstrained : forall i (rt:TypeRegisters) k_rs (k:DEX_ValKind) (r:DEX_Reg) (rs:DEX_Reg),
+      ~In r (locR p method_signature) ->
+      Some k_rs = BinNatMap.get _ rt rs ->
+      texec i (Move k r rs) None rt
+        (Some (BinNatMap.update _ rt r ((se i) U' k_rs)))
+
+    | moveResult_constrained : forall i (rt:TypeRegisters) k_res (k:DEX_ValKind) (r:DEX_Reg),
+      In r (locR p method_signature) ->
+      Some k_res = BinNatMap.get _ rt DEX_Registers.ret ->
+      se i <= sgn.(DEX_lvt) r ->
+      k_res <= sgn.(DEX_lvt) r ->
+      texec i (MoveResult k r) None rt
+        (Some (BinNatMap.update _ rt r ((se i) U' k_res)))
+
+    | moveResult_unconstrained : forall i (rt:TypeRegisters) k_res (k:DEX_ValKind) (r:DEX_Reg),
+      ~In r (locR p method_signature) ->
+      Some k_res = BinNatMap.get _ rt DEX_Registers.ret ->
+      texec i (MoveResult k r) None rt
+        (Some (BinNatMap.update _ rt r ((se i) U' k_res)))
+
+    | return_ : forall i (rt:TypeRegisters),
+      sgn.(DEX_resType) = None ->
+      texec i (Return) None rt None
+
+    | vReturn : forall i (rt:TypeRegisters) k_r kv (k:DEX_ValKind) (r:DEX_Reg),
+      Some k_r = BinNatMap.get _ rt r ->
+      sgn.(DEX_resType) = Some kv ->
+      ((se i) U' k_r) <=' kv ->
+      texec i (VReturn k r) None rt None
+
+    | const : forall i (rt:TypeRegisters) (k:DEX_ValKind) (r:DEX_Reg) (v:Z),
+      texec i (Const k r v) None rt (Some (BinNatMap.update _ rt r (L.Simple (se i))))
+    
+    | instanceOf : forall i (rt:TypeRegisters) k (r:DEX_Reg) (ro:DEX_Reg) (t:DEX_refType),
+      Some k = BinNatMap.get _ rt ro ->
+      (forall j, region i None j -> k <= se j) -> 
+      texec i (InstanceOf r ro t) None rt 
+        (Some (BinNatMap.update _ rt r (L.Simple ((se i) U k))))
+    
+    | arrayLength : forall i k ke (rt:TypeRegisters) (r:DEX_Reg) (rs:DEX_Reg),
+      Some (L.Array k ke) = BinNatMap.get _ rt rs ->
+      texec i (ArrayLength r rs) None rt
+        (Some (BinNatMap.update _ rt r (L.Simple k)))
+    
+    | new : forall i (rt:TypeRegisters) (r:DEX_Reg) (t:DEX_refType),
+      texec i (New r t) None rt (Some (BinNatMap.update _ rt r (L.Simple (se i))))
+
+    | newArray : forall i (rt:TypeRegisters) k (r:DEX_Reg) (rl:DEX_Reg) (t:DEX_type),
+      Some k = BinNatMap.get _ rt rl ->
+      texec i (NewArray r rl t) None rt
+        (Some (BinNatMap.update _ rt r (L.Array k (DEX_newArT p (m,i)))))
+
+    | goto : forall i (rt:TypeRegisters) (o:DEX_OFFSET.t),
+      texec i (Goto o) None rt (Some rt)
+
+    | packedSwitch : forall i k (rt:TypeRegisters) (r:DEX_Reg) (firstKey:Z) (size:Z) (l:list DEX_OFFSET.t),
+      Some k = BinNatMap.get _ rt r ->
+      (forall j, region i None j -> k <= se j) -> 
+      texec i (PackedSwitch r firstKey size l) None rt (Some (lift_rt k rt))
+
+    | sparseSwitch : forall i k (rt:TypeRegisters) (r:DEX_Reg) (size:Z) (l:list (Z * DEX_OFFSET.t)),
+      Some k = BinNatMap.get _ rt r ->
+      (forall j, region i None j -> k <= se j) -> 
+      texec i (SparseSwitch r size l) None rt (Some (lift_rt k rt))
+    
+    | ifcmp : forall i k (rt:TypeRegisters) (cmp:DEX_CompInt) (ra:DEX_Reg) (rb:DEX_Reg) (o:DEX_OFFSET.t),
+      Some k = BinNatMap.get _ rt ra ->
+      (forall j, region i None j -> k <= se j) -> 
+      texec i (Ifcmp cmp ra rb o) None rt (Some (lift_rt k rt))
+     
+    | ifz : forall i k (rt:TypeRegisters) (cmp:DEX_CompInt) (r:DEX_Reg) (o:DEX_OFFSET.t),
+      Some k = BinNatMap.get _ rt r ->
+      (forall j, region i None j -> k <= se j) -> 
+      texec i (Ifz cmp r o) None rt (Some (lift_rt k rt))
+
+    | aget : forall i ka kc ki (rt:TypeRegisters) 
+       (k:DEX_ArrayKind) (r:DEX_Reg) (ra:DEX_Reg) (ri:DEX_Reg),
+      Some (L.Array ka kc) = BinNatMap.get _ rt ra ->
+      Some ki = BinNatMap.get _ rt ri ->
+      texec i (Aget k r ra ri) None rt 
+        (Some (BinNatMap.update _ rt r ((ka U ki) U' kc)))
+
+    | aput : forall i ks ka kc ki (rt:TypeRegisters)
+       (k:DEX_ArrayKind) (rs:DEX_Reg) (ra:DEX_Reg) (ri:DEX_Reg),
+      Some ks = BinNatMap.get _ rt rs ->
+      Some (L.Array ka kc) = BinNatMap.get _ rt ra ->
+      Some ki = BinNatMap.get _ rt ri ->
+      ((ka U ki) U' ks) <=' kc ->
+      texec i (Aput k rs ra ri) None rt (Some rt)
+
+    | iget : forall i ko (rt:TypeRegisters) (k:DEX_ValKind) (r:DEX_Reg) (ro:DEX_Reg) (f:DEX_FieldSignature),
+      Some ko = BinNatMap.get _ rt ro ->
+      texec i (Iget k r ro f) None rt 
+        (Some (BinNatMap.update _ rt ro ((ko U (se i)) U' (DEX_ft p f))))
+
+    | iput : forall i ks ko (rt:TypeRegisters) (k:DEX_ValKind) (rs:DEX_Reg) (ro:DEX_Reg) (f:DEX_FieldSignature),
+      Some ks = BinNatMap.get _ rt rs ->
+      Some ko = BinNatMap.get _ rt ro ->
+      ((se i) U ko) U' ks <=' (DEX_ft p f) ->
+      texec i (Iput k rs ro f) None rt (Some rt)
+
+(*    | Sget (k:ValKind) (rt:Var) (f:FieldSignature)
+    | Sput (k:ValKind) (rs:Var) (f:FieldSignature) *)
+
+    | invokevirtual : forall i ko (rt:TypeRegisters) (m:DEX_MethodSignature) (n:Z) (par:list DEX_Reg),
+      length par = length (DEX_METHODSIGNATURE.parameters (snd m)) ->
+      compat_type_rt_lvt (DEX_virtual_signature p (snd m) ko) (rt) (par) (Z.to_nat n) ->
+      ko <= (DEX_virtual_signature p (snd m) ko).(DEX_heapEffect) -> 
+      sgn.(DEX_heapEffect) <= (DEX_virtual_signature p (snd m) ko).(DEX_heapEffect) ->
+      (* DEX *) (se i) <= (DEX_virtual_signature p (snd m) ko).(DEX_heapEffect) ->
+      compat_op (DEX_METHODSIGNATURE.result (snd m)) (DEX_virtual_signature p (snd m) ko).(DEX_resType) -> 
+      texec i (Invokevirtual m n par) None rt
+      (Some (update_op rt DEX_Registers.ret
+            (join_op (ko U (se i)) (DEX_virtual_signature p (snd m) ko).(DEX_resType)) ))
+(*
+    | Invokesuper (m:MethodSignature) (n:Z) (p:list Var)
+    | Invokedirect (m:MethodSignature) (n:Z) (p:list Var)
+*)
+    | invokestatic : forall i (rt:TypeRegisters) (m:DEX_MethodSignature) (n:Z) (par:list DEX_Reg),
+      length par = length (DEX_METHODSIGNATURE.parameters (snd m)) ->
+      compat_type_rt_lvt (DEX_static_signature p (snd m)) (rt) (par) (Z.to_nat n) ->
+      se i <= (DEX_static_signature p (snd m)).(DEX_heapEffect) -> 
+      sgn.(DEX_heapEffect) <= (DEX_static_signature p (snd m)).(DEX_heapEffect) ->
+      compat_op (DEX_METHODSIGNATURE.result (snd m)) (DEX_static_signature p (snd m)).(DEX_resType) -> 
+      texec i (Invokestatic m n par) None rt
+      (Some (update_op rt DEX_Registers.ret
+            (join_op (se i) (DEX_static_signature p (snd m)).(DEX_resType)) ))
+(*
+    | Invokeinterface (m:MethodSignature) (n:Z) (p:list Var)
+*)
+    | ineg : forall i ks (rt:TypeRegisters) (r:DEX_Reg) (rs:DEX_Reg),
+      Some ks = BinNatMap.get _ rt rs ->
+      texec i (Ineg r rs) None rt (Some (BinNatMap.update _ rt r (L.Simple ((se i) U ks))))
+
+    | inot : forall i ks (rt:TypeRegisters) (r:DEX_Reg) (rs:DEX_Reg),
+      Some ks = BinNatMap.get _ rt rs ->
+      texec i (Inot r rs) None rt (Some (BinNatMap.update _ rt r (L.Simple ((se i) U ks))))
+
+    | i2b : forall i ks (rt:TypeRegisters) (r:DEX_Reg) (rs:DEX_Reg),
+      Some ks = BinNatMap.get _ rt rs ->
+      texec i (I2b r rs) None rt (Some (BinNatMap.update _ rt r (L.Simple ((se i) U ks))))
+
+    | i2s : forall i ks (rt:TypeRegisters) (r:DEX_Reg) (rs:DEX_Reg),
+      Some ks = BinNatMap.get _ rt rs ->
+      texec i (I2s r rs) None rt (Some (BinNatMap.update _ rt r (L.Simple ((se i) U ks))))
+
+    | ibinop : forall i ka kb (rt:TypeRegisters) (op:DEX_BinopInt) (r:DEX_Reg) (ra:DEX_Reg) (rb:DEX_Reg),
+      Some ka = BinNatMap.get _ rt ra ->
+      Some kb = BinNatMap.get _ rt rb ->
+      texec i (Ibinop op r ra rb) None rt 
+       (Some (BinNatMap.update _ rt r (L.Simple ((ka U kb) U (se i)))))
+    
+    | ibinopConst : forall i ks (rt:TypeRegisters) (op:DEX_BinopInt) (r:DEX_Reg) (rs:DEX_Reg) (v:Z),
+      Some ks = BinNatMap.get _ rt rs ->
+      texec i (IbinopConst op r rs v) None rt 
+       (Some (BinNatMap.update _ rt r (L.Simple (ks U (se i)))))   
+    .
+
+    Section DEX_RT.
+      Variable RT : DEX_PC -> TypeRegisters.
+
+    Definition tsub_next (i:DEX_PC) rt : bool :=
+      match next m i with
+        | Some j => tsub_rt rt (RT j)
+        | None => false
+      end.
+
+(* DEX
+    Definition exception_test (i:PC) (e:ClassName) (k:L.t) : bool :=
+      match handler i e with
+        | Some t => tsub (L.Simple k::nil) (S t)
+        | None => L.leql_t k (sgn.(resExceptionType) e)
+      end.
+*)
+    Fixpoint in_test (e:DEX_ClassName) (l:list DEX_ClassName) : bool :=
+      match l with
+        | nil => false
+        | cn::q =>
+          (eqClassName e cn) || (in_test e q)
+      end.
+
+    Lemma In_in_test_true : forall e l,
+      In e l -> in_test e l = true.
+    Proof.
+      induction l; simpl; intros.
+      elim H.
+      destruct H; subst.
+      generalize (eqClassName_spec e e).
+      destruct (eqClassName e e) ; simpl; auto.
+      rewrite IHl; auto.
+      destruct (eqClassName e a) ; simpl; auto.
+    Qed.
+
+    Ltac clean_in_test :=
+      try match goal with
+        [ id1 : In ?e ?l, id2 : context[in_test ?e ?l = true] |- _ ] =>
+          rewrite (In_in_test_true e l id1) in id2
+      | [ id2 : context[in_test ?e ?l] |- _ ] =>
+          rewrite (In_in_test_true e l) in id2; [idtac|assumption]
+      end.
+
+(* DEX
+    Definition exception_test' (i:PC) (e:ClassName) (k:L.t) : bool :=
+      if in_test e (throwableAt m i) then
+        match handler i e with
+          | Some t => tsub (L.Simple k::nil) (S t)
+          | None => L.leql_t k (sgn.(resExceptionType) e)
+        end
+        else true.
+*)
+
+    Fixpoint tcompat_type_rt_lvt_aux (s:DEX_sign) (rt:TypeRegisters) 
+      (p:list DEX_Reg) (n:nat) {struct n} : bool :=
+      match n with (* could be optimised *)
+        | O => true
+        | Datatypes.S q => 
+          match nth_error p (q)%nat with
+          | None => false
+          | Some x =>
+            match BinNatMap.get _ rt x with
+            | None => false
+            | Some k => leql'_test k (DEX_lvt s (N_toReg (q)%nat))
+            end && tcompat_type_rt_lvt_aux s rt p q
+          end
+      end.
+
+    Lemma tcompat_type_rt_lvt_aux_true : forall s rt p n,
+      tcompat_type_rt_lvt_aux s rt p n = true ->
+      forall x, ((Reg_toN x)<n)%nat -> exists r k,
+        nth_error p (Reg_toN x) = Some r /\ BinNatMap.get _ rt r = Some k /\
+        L.leql' k (DEX_lvt s x).
+    Proof.
+      induction n. simpl.
+      intros.
+      apply False_ind; omega. simpl.
+
+      caseeq (nth_error p0 n); intros.
+      elim andb_prop with (1:=H0); clear H0; intros.
+      destruct (BinNatMap.get t' rt d) eqn:H3; intros.
+      elim (eq_excluded_middle _ (Reg_toN x) n); intros; subst.
+      (* replace (n0 - Reg_toN x - 1)%nat with (n0 - S (Reg_toN x))%nat. *)
+      exists d; exists t0; split; auto. (* Hendra *)
+      split; auto.
+      generalize (leql'_test_prop t0 (DEX_lvt s (N_toReg (Reg_toN x)))); rewrite H0. (* Hendra *)
+      rewrite Reg_toN_bij1; auto. 
+      apply IHn; auto. omega.
+      inversion H0.
+      inversion H0.
+    Qed.
+
+    Definition tcompat_type_rt_lvt (s:DEX_sign) (rt:TypeRegisters) (par:list DEX_Reg)
+      (n:nat) : bool := tcompat_type_rt_lvt_aux s rt par n.
+
+    Lemma tcompat_type_rt_lvt_true : forall s rt par n,
+      tcompat_type_rt_lvt s rt par n = true ->
+      compat_type_rt_lvt s rt par n.
+    Proof.
+      unfold tcompat_type_rt_lvt, compat_type_rt_lvt; intros.
+      apply (tcompat_type_rt_lvt_aux_true _ _ _ _ H); auto.
+    Qed.
+
+    Definition tcompat_op (ot:option DEX_type) (ok:option L.t') : bool :=
+      match ot,ok with
+        | None,None => true
+        | Some _,Some _ => true
+        | _,_ => false
+      end.
+
+    Lemma tcompat_op_true : forall (ot:option DEX_type) (ok:option L.t'),
+      tcompat_op ot ok = true -> compat_op ot ok.
+    Proof.
+      destruct ot; destruct ok; simpl; intros; discriminate || constructor.
+    Qed.
+
+(* DEX
+    Fixpoint pop_n (A:Type) (n:nat) (l:list A) {struct n} : list A :=
+      match n with
+        | O => l
+        | Datatypes.S p => match l with
+                   | nil => nil
+                   | x::q => pop_n A p q
+                 end
+      end.
+    Implicit Arguments pop_n [A].
+
+    Lemma pop_n_length_fst : forall A (l1 l2:list A),
+      pop_n (length l1) (l1 ++ l2) = l2.
+    Proof.
+      induction l1; simpl; auto.
+    Qed.
+*)
+    Fixpoint le_nat_test (n1 n2:nat) {struct n1} : bool :=
+       match n1 with
+         | O => true
+         | Datatypes.S p1 =>
+             match n2 with
+               | O => false
+               | Datatypes.S p2 => le_nat_test p1 p2
+             end
+       end.
+
+    Lemma le_nat_test_correct : forall n1 n2,
+      if le_nat_test n1 n2 then (n1<=n2)%nat else (~(n1<=n2))%nat.
+    Proof.
+      induction n1; simpl.
+      intros; omega.
+      destruct n2; simpl.
+      omega.
+      generalize (IHn1 n2); destruct (le_nat_test n1 n2); omega.
+    Qed.
+
+    Lemma le_nat_test_true : forall n1 n2,
+      le_nat_test n1 n2 = true -> (n1<=n2)%nat.
+    Proof.
+      intros.
+      generalize (le_nat_test_correct n1 n2).
+      rewrite H; auto.
+    Qed.
+
+(* Duplicate with the one in Annotated.v? 
+    Definition compat_type_rt_lvt (s:sign) (rt:TypeRegisters) (n:nat) : Prop :=
+      forall x, ((Reg_toN x)<n)%nat -> exists k,
+        nth_error st (n-(Var_toN x)-1)%nat = Some k /\
+        L.leql' k (lvt s x).
+*)
+
+   Definition tcheck (i:DEX_PC) (ins:DEX_Instruction) : bool :=
+      match ins,S i with
+        | Aconst_null,   st1 => 
+          tsub_next i (L.Simple (se i)::st1)
+        | Arraylength,   (L.Array k ke::st) =>
+          (selift i None k) &&
+          (tsub_next i (L.Simple k::(elift m i k st))) &&
+          for_all _
+            (fun e => (selift i (Some e) k) && (exception_test i e k))
+            (throwableAt m i)
+        | Athrow,        (L.Simple k::st) =>
+          for_all _
+            (fun e => (selift i (Some e) k) && (exception_test i e k))
+            (throwableAt m i)
+        | Checkcast _,   k::st =>
+          (selift i None k) &&
+          (tsub_next i (k::elift m i k st)) &&
+          for_all _
+            (fun e => (selift i (Some e) k) && (exception_test i e k))
+            (throwableAt m i)
+        | Const _ _,       st =>
+          tsub_next i (L.Simple (se i)::st) 
+        | Dup,             k::st =>
+          tsub_next i (k::k::st)
+        | Dup_x1,          k1::k2::st =>
+          tsub_next i (k1::k2::k1::st) 
+        | Dup_x2,          k1::k2::k3::st =>
+          tsub_next i (k1::k2::k3::k1::st) 
+        | Dup2,            k1::k2::st =>
+          tsub_next i (k1::k2::k1::k2::st) 
+        | Dup2_x1,         k1::k2::k3::st =>
+          tsub_next i (k1::k2::k3::k1::k2::st) 
+        | Dup2_x2,         k1::k2::k3::k4::st =>
+          tsub_next i (k1::k2::k3::k4::k1::k2::st) 
+        | Getfield f,      L.Simple k::st =>
+          (selift i None k) &&
+          (tsub_next i ((k U' (ft p f))::(elift m i k st))) &&
+          for_all _
+            (fun e => (selift i (Some e) k) && (exception_test i e k))
+            (throwableAt m i)
+        | Goto o,          st =>
+          tsub st (S (OFFSET.jump i o)) 
+        | I2b,             L.Simple k::st =>
+          tsub_next i (L.Simple k::st) 
+        | I2s,             L.Simple k::st =>
+          tsub_next i (L.Simple k::st) 
+        | Ibinop DivInt,       L.Simple k1::L.Simple k2::st =>
+          (selift i None k1) &&
+          (tsub_next i (L.Simple (L.join k1 k2)::(elift m i k1 st))) &&
+          for_all _
+            (fun e => (selift i (Some e) k1) && (exception_test i e k1))
+            (throwableAt m i)
+        | Ibinop RemInt,       L.Simple k1::L.Simple k2::st =>
+          (selift i None k1) &&
+          (tsub_next i (L.Simple (L.join k1 k2)::(elift m i k1 st))) &&
+          for_all _
+            (fun e => (selift i (Some e) k1) && (exception_test i e k1))
+            (throwableAt m i)
+        | Ibinop _,       L.Simple k1::L.Simple k2::st =>
+          tsub_next i (L.Simple (L.join k1 k2)::st)
+        | If_acmp _ o,    L.Simple k1::L.Simple k2::st =>
+          (selift i None (L.join k1 k2)) &&
+          (tsub_next i (lift (L.join k1 k2) st)) &&
+          (tsub (lift (L.join k1 k2) st) (S (OFFSET.jump i o)))
+        | If_icmp _ o,    L.Simple k1::L.Simple k2::st =>
+          (selift i None (L.join k1 k2)) &&
+          (tsub_next i (lift (L.join k1 k2) st)) &&
+          (tsub (lift (L.join k1 k2) st) (S (OFFSET.jump i o)))
+        | If0 _ o,        L.Simple k::st =>
+          (selift i None k) &&
+          (tsub_next i (lift k st)) &&
+          (tsub (lift k st) (S (OFFSET.jump i o)))
+        | Ifnull _ o,        k::st =>
+          (selift i None k) &&
+          (tsub_next i (lift k st)) &&
+          (tsub (lift k st) (S (OFFSET.jump i o)))
+        | Iinc x c,         st =>
+          (L.leql_t (se i) (sgn.(lvt) x)) &&
+          (tsub_next i st)
+        | Ineg,             k::st =>
+          tsub_next i (k::st)
+        | Instanceof _,     k::st =>
+          (selift i None k) &&
+          (tsub_next i (k::st))
+        | Invokestatic mid, st =>
+          let n := length (METHODSIGNATURE.parameters (snd mid)) in
+          let sgn' := (static_signature p (snd mid)) in 
+          let ke' := (join_list sgn'.(resExceptionType) (throwableBy p (snd mid))) in
+            le_nat_test n (length st) &&
+            (tcompat_type_st_lvt (static_signature p (snd mid)) st n) &&
+            (L.leql_t (se i) sgn'.(heapEffect)) &&
+            (selift i None ke') &&
+            for_all _
+              (fun e => (selift i (Some e) (sgn'.(resExceptionType) e) &&
+                        (exception_test i e (L.join (se i) (sgn'.(resExceptionType) e)))) &&
+                        (L.leql_t (se i) (sgn.(resExceptionType) e))) 
+              (throwableBy p (snd mid)) &&
+            (tcompat_op (METHODSIGNATURE.result (snd mid)) sgn'.(resType)) &&
+            (L.leql_t sgn.(heapEffect) sgn'.(heapEffect)) && 
+            tsub_next i (lift ke' (cons_option (join_op (se i) sgn'.(resType)) (pop_n n st)))
+        | Invokevirtual mid, st =>
+          let n := length (METHODSIGNATURE.parameters (snd mid)) in
+            match pop_n n st with
+              | (L.Simple k1)::st2 =>
+                le_nat_test (Datatypes.S n) (length st) &&
+                (tcompat_type_st_lvt (virtual_signature p (snd mid) k1) st (Datatypes.S n)) &&
+                (L.leql_t k1 (virtual_signature p (snd mid) k1).(heapEffect)) &&
+                (selift i None (L.join (join_list (virtual_signature p (snd mid) k1).(resExceptionType) (throwableBy p (snd mid))) k1)) &&
+                (for_all _
+                  (fun cn => 
+                    (selift i (Some cn) (L.join ((virtual_signature p (snd mid) k1).(resExceptionType) cn) k1)) &&
+                    (exception_test i cn (L.Simple (L.join k1 ((virtual_signature p (snd mid) k1).(resExceptionType) cn)))) &&
+                    (L.leql_t k1 (sgn.(resExceptionType) cn)) &&
+                    (L.leql_t ((virtual_signature p (snd mid) k1).(resExceptionType) cn) (sgn.(resExceptionType) cn)))
+                  (throwableAt m i ++ throwableBy p (snd mid))) &&
+                (tcompat_op (METHODSIGNATURE.result (snd mid)) (virtual_signature p (snd mid) k1).(resType)) &&
+                (L.leql_t sgn.(heapEffect) (virtual_signature p (snd mid) k1).(heapEffect)) &&
+                tsub_next i (lift k1 (lift (join_list (virtual_signature p (snd mid) k1).(resExceptionType) (throwableBy p (snd mid))) 
+                  (cons_option (join_op k1 (virtual_signature p (snd mid) k1).(resType)) st2)))
+              | _ => false
+            end
+        | Lookupswitch d l, L.Simple k::st =>
+          (selift i None k) &&
+          (for_all _
+            (fun o => tsub (lift k st) (S (OFFSET.jump i o)))
+            (d::@map _ _ (@snd _ _) l)) &&
+          tsub_next i (lift k st)
+        | New c, st =>
+          tsub_next i (L.Simple (se i)::st)
+        | Newarray t, (L.Simple k::st) =>
+          (selift i None k) &&
+          tsub_next i (L.Array k (newArT p (m,i))::elift m i k st) &&
+          for_all _
+            (fun e => (selift i (Some e) k) && (exception_test i e k))
+            (throwableAt m i)
+        | Nop, st => tsub_next i st
+        | Pop, k::st => tsub_next i  st
+        | Pop2, k1::k2::st => tsub_next i st
+        | Putfield f, (k1::L.Simple k2::st) =>
+          leql'_test k1 (ft p f) &&
+          L.leql_t k2 (ft p f) &&
+          L.leql_t (se i) (ft p f) &&
+          L.leql_t sgn.(heapEffect) (ft p f) &&
+          selift i None k2 &&
+          tsub_next i (elift m i k2 st) &&
+          for_all _
+            (fun e => (selift i (Some e) k2) && (exception_test i e k2))
+            (throwableAt m i)
+        | Return, st =>
+          match sgn.(resType) with
+            | None => true
+            | _ => false
+          end
+        | Swap, k1::k2::st => tsub_next i (k2::k1::st)
+        | Tableswitch d lo hi l, L.Simple k::st =>
+          (selift i None k) &&
+          (tsub_next i (lift k st)) &&
+          (for_all _
+            (fun o => tsub (lift k st) (S (OFFSET.jump i o)))
+            (d::l))          
+        | Vaload t, L.Simple k1::L.Array k2 ke::st =>
+          (selift i None k2) &&
+          (selift i None (L.join k1 k2)) &&
+          (tsub_next i (L.join' (L.join k1 k2) ke::elift m i (L.join k1 k2) st)) &&
+          (selift i (Some np) k2) && (exception_test' i np k2) &&
+          (selift i (Some iob) (k1 U k2)) && (exception_test' i iob (k1 U k2)) 
+        | Vastore t, kv::L.Simple ki::L.Array ka ke::st =>
+          (leql'_test kv ke) &&
+          (L.leql_t ki ke) &&
+          (L.leql_t ka ke) &&
+          (selift i None ka) &&
+          (selift i None (L.join ki ka)) &&
+          (selift i None ke) &&
+          (L.leql_t (heapEffect sgn) ke) &&
+          (tsub_next i (elift m i ke st)) &&
+          (selift i (Some np) ka) && (exception_test' i np ka) &&
+          (selift i (Some ase) (L.join kv (L.join ki ka))) && (exception_test' i ase (L.join kv (L.join ki ka))) && 
+          (selift i (Some iob) (L.join ki ka)) && (exception_test' i iob (L.join ki ka)) 
+        | Vload t x, st =>
+          tsub_next i (L.join' (se i) (sgn.(lvt) x)::st)
+        | Vstore t x, k::st =>
+          L.leql_t (se i) (sgn.(lvt) x) &&
+          leql'_test k (sgn.(lvt) x) &&
+          tsub_next i st
+        | Vreturn x, k::st =>
+          match sgn.(resType) with
+            | None => false
+            | Some kv => leql'_test k kv 
+          end
+        | _,_ => false      end.
+
+   Ltac flatten_bool :=
+     repeat match goal with
+       [ id : _ && _ = true |- _ ] =>  destruct (andb_prop _ _ id); clear id
+     end.
+
+   Variable selift_prop : forall i tau k,
+     selift i tau k = true ->
+     forall j, region i tau j -> k <= (se j).
+
+   Ltac replace_selift :=
+     repeat match goal with
+       [ id : selift _ _ _ = true |- _ ] =>  
+         generalize (selift_prop _ _ _ id);
+           clear id; intros id
+     end.
+
+   Lemma leql_prop : forall x y,
+     L.leql_t x y = true -> x <= y.
+   Proof.
+     intros.
+     generalize (L.leql_t_spec x y); rewrite H; auto.
+   Qed.
+
+   Ltac replace_leql :=
+     repeat match goal with
+       [ id : L.leql_t _ _ = true |- _ ] =>  
+         generalize (leql_prop _ _ id);
+           clear id; intros id
+     | [ id : leql'_test ?x ?y = true |- _ ] =>  
+       generalize (leql'_test_prop x y); rewrite id; clear id; intros id
+     end.
+
+   Ltac replace_for_all :=
+     match goal with
+       [ id1 : for_all _ _ ?l = true,
+         id2 : In ?e ?l |- _] =>
+       generalize (for_all_true _ _ _ id1 _ id2);
+         clear id1; intros id1
+     end.
+
+   Ltac replace_handler :=
+     repeat match goal with
+       [ id1 : StaticHandler.handler ?s ?m ?i ?e = _,
+         id2 : context[StaticHandler.handler ?s ?m ?i ?e] |- _ ] =>
+       rewrite id1 in id2
+     end.
+
+   Ltac flatten :=
+     flatten_bool; try replace_for_all; flatten_bool;
+       replace_handler; replace_selift; clean_in_test; replace_leql.
+
+   Lemma length_le_app_form : forall (A:Set) n (l:list A),
+     (n<= length l)%nat -> exists l1, exists l2,
+       l = l1++l2 /\ n = length l1.
+   Proof.
+     induction n; intros.
+     exists (@nil A); exists l; split; auto.
+     inversion H.
+     exists l; exists (@nil A); split; auto.
+     apply app_nil_end.
+     elim IHn with l.
+     intros l1 [l2 [H3 H2]].
+     destruct l2.
+     rewrite <- app_nil_end in H3; subst.
+     apply False_ind; omega.
+     exists (l1++(a::nil)); exists l2; split.
+     rewrite <- app_cons; auto.
+     rewrite length_app_cons_nil; congruence.
+     omega.
+   Qed.
+
+   Ltac split_match :=
+     repeat 
+       match goal with
+         | [ _ : context[match ?x with nil => _ | _ :: _ => _ end] |- _] => destruct x
+         | [ _ : context[match ?x with L.Simple _ => _ | L.Array _ _ => _ end] |- _] => destruct x
+         | [_ :  context [match ?x with
+                            | Make.AddInt => _
+                            | Make.AndInt => _
+                            | Make.DivInt => _
+                            | Make.MulInt => _
+                            | Make.OrInt => _
+                            | Make.RemInt => _
+                            | Make.ShlInt => _
+                            | Make.ShrInt => _
+                            | Make.SubInt => _
+                            | Make.UshrInt => _
+                            | Make.XorInt => _
+                          end] |- _] => destruct x
+       end.
+
+
+   Lemma tcheck_correct1 : forall i ins,
+     tcheck i ins = true ->
+     forall tau, step p subclass_test m i ins tau None ->
+       texec i ins tau (S i) None.
+   Proof.
+     intros.
+     inversion_clear H0 in H;
+       unfold tcheck, step.handler, exception_test, exception_test' in *;
+     try (destruct (S i) as [ | [|]]; intros; try discriminate; flatten;
+       constructor; auto).
+     destruct H2;subst;  split_match; intros; try discriminate.
+     (* Ibinop *)
+     split_match; intros; try discriminate; flatten.
+     constructor; auto.
+     split_match; intros; try discriminate; flatten.
+     constructor; auto.
+     (* Invokestatic *)
+     flatten_bool.
+     generalize (le_nat_test_true _ _ H0); clear H0; intros H0.
+     destruct (length_le_app_form _ _ _ H0) as [st1 [st2 [T1 T2]]].
+     rewrite T1.
+     constructor; flatten; auto.
+     apply tcompat_type_st_lvt_true.
+     congruence.
+     apply L.leql_trans with (2:=H11); apply L.join_right.
+     (* Invokevirtual *)
+     case_eq (pop_n  (length (METHODSIGNATURE.parameters (@snd ClassName METHODSIGNATURE.t mid))) (S i)).
+     intros HH; rewrite HH in H; flatten_bool.
+     discriminate.
+     intros k1 st2 HH; rewrite HH in H.
+     destruct k1 as [k1|]; try discriminate.
+     flatten_bool.
+     generalize (le_nat_test_true _ _ H0); clear H0; intros H0.
+     assert (length (METHODSIGNATURE.parameters (@snd ClassName METHODSIGNATURE.t mid)) <= length (S i))%nat.
+     omega.
+     destruct (length_le_app_form _ _ _ H) as [st1 [st3 [T1 T2]]].
+     rewrite T1.
+     rewrite T1 in HH; rewrite T2 in HH; rewrite pop_n_length_fst in HH.
+     subst.
+     flatten.
+     rewrite T1 in *.
+     constructor; flatten; auto.
+     apply tcompat_type_st_lvt_true.
+     rewrite <- T2; auto.
+     (* Putfield *)
+     destruct (S i) as [ | k1 l]; intros; try discriminate.
+     destruct l as [ | k2 l]; intros; try discriminate.
+     destruct k2 as [ k2 |]; intros; try discriminate.
+     flatten.
+     constructor; auto.
+     (* return*) 
+     destruct (resType sgn); congruence.
+     destruct (resType sgn); congruence.
+     destruct (resType sgn); congruence.
+     (* Vaload *)
+     destruct (S i) as [ |k1 l]; intros; try discriminate.
+     destruct k1 as [k1|]; try discriminate.
+     destruct l as [|k2 l]; try discriminate.
+     destruct k2 as [k2|]; try discriminate.
+     flatten.
+     constructor; auto.
+     auto.
+replace_leql.
+     auto.
+
+     destruct (S i) as [ |k1 l]; intros; try discriminate.
+     destruct k1 as [k1|]; try discriminate.
+     destruct l as [|k2 l]; try discriminate.
+     destruct k2 as [k2|]; try discriminate.
+     flatten.
+     constructor; auto.
+     rewrite (In_in_test_true _ _ H1) in *; flatten; auto.
+
+     (* Vastore *)
+     destruct (S i) as [ |kv l]; intros; try discriminate.
+     destruct l as [|k2 l]; try discriminate.
+     destruct k2 as [ki|]; try discriminate.
+     destruct l as [|k2 l]; try discriminate.
+     destruct k2 as [|ka ke]; try discriminate.
+     flatten.
+     constructor; auto.
+     rewrite (In_in_test_true _ _ H1) in *; flatten; auto.
+   
+     destruct (S i) as [ |kv l]; intros; try discriminate.
+     destruct l as [|k2 l]; try discriminate.
+     destruct k2 as [ki|]; try discriminate.
+     destruct l as [|k2 l]; try discriminate.
+     destruct k2 as [|ka ke]; try discriminate.
+     flatten.
+     constructor; auto.
+     rewrite (In_in_test_true _ _ H1) in *; flatten; auto.
+
+     destruct (S i) as [ |kv l]; intros; try discriminate.
+     destruct l as [|k2 l]; try discriminate.
+     destruct k2 as [ki|]; try discriminate.
+     destruct l as [|k2 l]; try discriminate.
+     destruct k2 as [|ka ke]; try discriminate.
+     flatten.
+     econstructor; eauto.
+     (* Vreturn *)
+     destruct (S i) as [ |k l]; intros; try discriminate.
+     generalize H; clear H; case_eq (resType sgn); intros; try discriminate.
+     econstructor; eauto.
+     generalize (leql'_test_prop k t0). (* Hendra *)
+     rewrite H0; auto.
+   Qed.
+
+   Ltac replace_tsub_next :=
+     try match goal with
+       [ id1 : tsub_next _ ?st = true, id2 : next _ _ = _ |- _ ] =>
+         unfold tsub_next in id1; rewrite id2 in id1
+     end.
+
+   Ltac search_tsub :=
+     match goal with
+       [ id1 : tsub ?st (S _) = true |- _ ] =>
+         exists st; split; [clear id1 | exact id1]
+         end.
+
+   Ltac flatten2 := flatten; replace_tsub_next; search_tsub.
+
+   Hint Constructors texec : texec.
+
+   Lemma tcheck_correct2 : forall i ins,
+     tcheck i ins = true ->
+     forall tau j, step p subclass_test m i ins tau (Some j) ->
+       exists st,
+       texec i ins tau (S i) (Some st)
+       /\ tsub st (S j) = true.
+   Proof.
+     intros.
+     inversion_clear H0 in H;
+       unfold tcheck, step.handler, exception_test, exception_test' in *;
+     try (split_match; intuition; subst; try discriminate; flatten2; eauto with texec; fail).
+     split_match; intuition; try discriminate; flatten2.
+     apply arraylength_np_caught with (t := j). apply H0. apply H2.
+     
+     split_match; try (case op in H; inversion H; fail).
+     destruct op; flatten2; apply ibinop; auto.
+ 
+     (* invokestatic *)
+     flatten2.
+     elim length_le_app_form with (n:=(length (METHODSIGNATURE.parameters (snd mid)))) (l:=(S i)).
+     intros st1 [st2 [T1 T2]].
+     rewrite T1.
+     rewrite T2.
+     rewrite pop_n_length_fst.
+     constructor; auto.
+     rewrite <- T1; rewrite <- T2; apply tcompat_type_st_lvt_true; auto.
+     apply tcompat_op_true; auto.
+     generalize (le_nat_test_correct (length (METHODSIGNATURE.parameters (snd mid)))
+       (length (S i))); rewrite H0; auto.
+     (**)
+     flatten2.
+     elim length_le_app_form with (n:=(length (METHODSIGNATURE.parameters (@snd ClassName METHODSIGNATURE.t mid)))) (l:=(S i)).
+     intros st1 [st2 [T1 T2]].
+     rewrite T1.
+     constructor; auto.
+     rewrite <- T1; rewrite <- T2; apply tcompat_type_st_lvt_true; auto.
+     generalize (le_nat_test_correct (length (METHODSIGNATURE.parameters (@snd ClassName METHODSIGNATURE.t mid)))
+       (length (S i))).
+     rewrite H0; auto.
+     (* invokevirtual *)
+     generalize H; clear H.
+     case_eq (pop_n  (length (METHODSIGNATURE.parameters (@snd ClassName METHODSIGNATURE.t mid))) (S i)); intros.
+     discriminate. 
+     destruct t0 as [k1|]; try discriminate.
+     (*destruct t as [k1|]; try discriminate.*)
+     flatten2.
+     elim length_le_app_form with (n:=(length (METHODSIGNATURE.parameters (snd mid)))) (l:=(S i)).
+     intros st1 [st2 [T1 T2]].
+     rewrite T1.
+     rewrite T1 in H; rewrite T2 in H; rewrite pop_n_length_fst in H.
+     subst.
+     constructor; auto.
+     rewrite <- T1; rewrite <- T2; apply tcompat_type_st_lvt_true; auto.
+     apply tcompat_op_true; auto.
+     generalize (le_nat_test_true _ _ H2); clear H2; intros H2.
+     omega.
+     (**)
+     generalize H; clear H.
+     case_eq (pop_n  (length (METHODSIGNATURE.parameters (@snd ClassName METHODSIGNATURE.t mid))) (S i)); intros.
+     discriminate.
+     destruct t0 as [k1|]; try discriminate.
+     (*destruct t as [k1|]; try discriminate.*)
+     flatten.
+     elim length_le_app_form with (n:=(length (METHODSIGNATURE.parameters (@snd ClassName METHODSIGNATURE.t mid)))) (l:=(S i)).
+     intros st1 [st2 [T1 T2]].
+     rewrite T1.
+     rewrite T1 in H; rewrite T2 in H; rewrite pop_n_length_fst in H.
+     subst.
+     exists (lift k1 (L.Simple (L.join k1 ((virtual_signature p (snd mid) k1).(resExceptionType) e))::nil)).
+     split.
+     constructor; auto.
+     rewrite <- T1; rewrite <- T2; apply tcompat_type_st_lvt_true; auto.
+     simpl.
+     simpl in H13.
+     destruct (S j); try discriminate.
+     destruct t0; try discriminate.
+     (*destruct t; try discriminate.*)
+     flatten_bool.
+     destruct t1; try discriminate.
+     (*destruct t0; try discriminate.*)
+     replace_leql.
+     generalize (L.leql_t_spec (k1 U k1 U resExceptionType (virtual_signature p (snd mid) k1) e) k).
+     destruct (L.leql_t (k1 U k1 U resExceptionType (virtual_signature p (snd mid) k1) e) k); auto.
+     intros.
+     elim H13.
+     apply L.join_least.
+     apply L.leql_trans with (2:=H).
+     apply L.join_left.
+     auto.     
+     generalize (le_nat_test_true _ _ H3); clear H3; intros H3.
+     omega.
+     (* vaload *)
+   Qed.
+ End DEX_S.
+*)
+  End DEX_typing_rules.
+
+
