JVM_BigStepAnnot.v
@@ -1,0 +1,202 @@
+(** BigStepAnnot.v: We constrain the Bicolano bigstep semantics to handle only the executions where exception thrown at a given point are in a predefined set. Such a set could be computed for example with a CHA static analysis. *)
+Require Export List.
+Require Export ZArith.
+Require Export LoadBicolano.
+
+Inductive compat_op (A B:Set) : option A -> option B -> Prop :=
+  compat_op_none : compat_op A B None None
+| compat_op_some : forall k v, compat_op A B (Some k) (Some v).
+Implicit Arguments compat_op [A B].
+
+
+Module JVM_BigStepAnnot.
+
+Import JVM_BigStep.JVM_BigStep JVM_StaticHandler.JVM_StaticHandler JVM_Dom JVM_Prog.
+
+
+
+  Set Implicit Arguments.
+  Section JVM_instr.
+(* DEX
+  Variable throwableAt : Method -> PC -> list ClassName.
+  Variable throwableBy : ShortMethodSignature -> list ClassName.
+
+  Inductive ExceptionStep (p:Program) : Method -> IntraNormalState -> IntraExceptionState -> Prop :=
+  | athrow : forall h m pc s l loc cn,
+
+    instructionAt m pc = Some Athrow ->
+    Heap.typeof h loc = Some (Heap.LocationObject cn) ->
+    subclass_name p cn javaLangThrowable ->
+    In cn (throwableAt m pc) -> (* Specific hypothesis here *)
+    ExceptionStep p m (pc,(h,(Ref loc::s),l)) (h,loc)
+
+
+  | jvm_exception : forall h m pc s l h' loc (e:ShortClassName),
+
+    JVMExceptionStep p m (pc,(h,s,l)) e ->
+    Heap.new h p (Heap.LocationObject (javaLang,e)) = Some (loc,h') ->
+    In (javaLang,e) (throwableAt m pc) -> (* Specific hypothesis here *)
+
+    ExceptionStep p m (pc,(h,s,l)) (h',loc).
+*)
+
+  Inductive JVM_exec_intra (p:JVM_Program) (m:JVM_Method) : option JVM_ClassName -> JVM_IntraNormalState -> JVM_IntraNormalState -> Prop :=
+  | exec_intra_normal : forall s1 s2,
+    JVM_NormalStep p m s1 s2 ->
+    JVM_exec_intra p m None s1 s2
+  (* DEX | exec_exception : forall pc1 h1 h2 loc2 s1 l1 pc' e,
+    ExceptionStep p m (pc1,(h1,s1,l1)) (h2,loc2) ->
+    CaughtException p m (pc1,h2,loc2) pc' ->
+    Heap.typeof h2 loc2 = Some (Heap.LocationObject e) ->
+    exec_intra p m (Some e) (pc1,(h1,s1,l1)) (pc',(h2,Ref loc2::OperandStack.empty,l1))*).
+
+  Inductive JVM_exec_return (p:JVM_Program) (m:JVM_Method) : option JVM_ClassName -> JVM_IntraNormalState -> JVM_ReturnState -> Prop :=
+  | exec_return_normal : forall s h ov,
+     JVM_ReturnStep p m s (h,Normal ov) ->
+     JVM_exec_return p m None s (h,Normal ov)
+  (* DEX | exec_return_exception : forall pc1 h1 h2 loc2 s1 l1 e,
+     ExceptionStep p m (pc1,(h1,s1,l1)) (h2,loc2) ->
+     UnCaughtException  p m (pc1,h2,loc2) ->
+     Heap.typeof h2 loc2 = Some (Heap.LocationObject e) ->
+     exec_return p m (Some e) (pc1,(h1,s1,l1)) (h2,Exception loc2)*) .
+
+  Inductive JVM_exec_call (p:JVM_Program)  (m:JVM_Method) : option JVM_ClassName ->
+   JVM_IntraNormalState -> JVM_ReturnState -> JVM_Method  -> JVM_IntraNormalState -> JVM_IntraNormalState + JVM_ReturnState  -> Prop :=
+ | exec_call_normal : forall m2 pc1 pc1' h1 s1 l1 os l2 h2 bm2 ov,
+     JVM_CallStep p m (pc1,(h1,s1,l1 )) (m2,(os,l2)) ->
+     JVM_METHOD.body m2 = Some bm2 ->
+     next m pc1 = Some pc1' ->
+     compat_op ov (JVM_METHODSIGNATURE.result (JVM_METHOD.signature m2)) ->
+     JVM_exec_call p m None
+        (pc1,(h1,s1,l1))
+        (h2,Normal ov)
+        m2
+        (JVM_BYTECODEMETHOD.firstAddress bm2,(h1,JVM_OperandStack.empty,l2))
+        (inl _ (pc1',(h2,cons_option ov os,l1)))
+(* DEX
+ | exec_call_caught : forall m2 pc1 pc1' h1 s1 l1 os l2 h2 loc bm2 cn,
+     CallStep p m (pc1,(h1,s1,l1 )) (m2,(os,l2)) ->
+     METHOD.body m2 = Some bm2 ->
+     CaughtException p m (pc1, h2, loc) pc1' ->
+
+     Heap.typeof h2 loc = Some (Heap.LocationObject cn) ->
+     In cn (throwableBy (METHOD.signature m2)) -> (* Specific hypothesis here *)
+
+     exec_call p m (Some cn)
+        (pc1,(h1,s1,l1))
+        (h2,Exception loc)
+        m2
+        (BYTECODEMETHOD.firstAddress bm2,(h1,OperandStack.empty,l2))
+        (inl _(pc1',(h2,Ref loc::nil,l1)))
+ | exec_call_uncaught : forall m2 pc1 h1 s1 l1 os l2 h2 loc bm2 cn,
+     CallStep p m (pc1,(h1,s1,l1 )) (m2,(os,l2)) ->
+     METHOD.body m2 = Some bm2 ->
+     UnCaughtException p m (pc1, h2, loc)  ->
+
+     Heap.typeof h2 loc = Some (Heap.LocationObject cn) ->
+     In cn (throwableBy (METHOD.signature m2)) -> (* Specific hypothesis here *)
+
+     exec_call p m (Some cn)
+       (pc1,(h1,s1,l1))
+       (h2,Exception loc)
+       m2
+       (BYTECODEMETHOD.firstAddress bm2,(h1,OperandStack.empty,l2))
+       (inr _ (h2,Exception loc))*) .
+
+ Inductive JVM_IntraStep (p:JVM_Program) : 
+    JVM_Method -> JVM_IntraNormalState -> JVM_IntraNormalState + JVM_ReturnState -> Prop :=
+  | IntraStep_res :forall m s ret tau,
+     JVM_exec_return p m tau s ret ->
+     JVM_IntraStep p m s (inr _ ret)
+  | IntraStep_intra_step:forall m s1 s2 tau,
+     JVM_exec_intra p m tau s1 s2 ->
+     JVM_IntraStep p m s1 (inl _ s2) 
+  | IntraStep_call :forall m m' s1 s' ret' r tau,
+     JVM_exec_call p m tau s1 ret' m' s' r ->
+     TransStep_l (JVM_IntraStep p m') s' (inr _ ret') ->
+     JVM_IntraStep p m s1 r.
+ 
+ Definition JVM_IntraStepStar p m s r := TransStep_l (JVM_IntraStep p m) s r.
+
+ Definition JVM_IntraStepStar_intra p m s s' := JVM_IntraStepStar p m s (inl _ s').
+
+ Definition JVM_BigStep  p m s ret := JVM_IntraStepStar p m s (inr _ ret).
+
+
+  Lemma JVM_IntraStep_ind_ : 
+      forall (p:JVM_Program) 
+        (P:JVM_Method->JVM_IntraNormalState->JVM_IntraNormalState+JVM_ReturnState->Prop),
+         (forall m s, P m s (inl _ s)) ->
+         (forall m tau s r, JVM_exec_return p m tau s r -> P m s (inr _ r)) ->
+         (forall m tau s s' , JVM_exec_intra p m tau s s' -> 
+            forall r, JVM_IntraStepStar p m s' r -> P m s' r ->
+            P m s r) ->
+         (forall m tau s s' ret m' r, 
+            JVM_exec_call p m tau s ret m' s' (inr _ r) ->
+            JVM_IntraStepStar p m' s' (inr _ ret) ->
+            P m' s' (inr _ ret) ->
+            P m s (inr _ r)) ->
+         (forall m tau s s' ret m' s'' r, 
+            JVM_exec_call p m tau s ret m' s' (inl _ s'') ->
+            JVM_IntraStepStar p m' s' (inr _ ret) -> P m' s' (inr _ ret) ->
+            JVM_IntraStepStar p m s'' r -> P m s'' r ->
+            P m s r) ->
+      forall m s r, JVM_IntraStep p m s r -> 
+        match r with
+        | inr r' => P m s (inr _ r')
+        | inl s' => forall r', JVM_IntraStepStar p m s' r' -> P m s' r' -> P m s r'
+        end.
+     Proof.
+       intros prg Q H0 Hr Hi Hcr Hc.
+       fix intra 4;intros m s r Hs;case Hs;clear m s r Hs;intros.
+       eapply Hr; eauto.
+       apply Hi with tau s2;trivial. 
+       assert (Q m' s' (inr JVM_IntraNormalState ret')).
+       generalize s' (inr JVM_IntraNormalState ret') H1;clear H1 H m s1 s' ret' r.
+       fix fixp 3;intros s' s Ht;case Ht;clear Ht s' s;intros.
+       apply H0.
+       generalize (intra _ _ _ H);clear H;case r;intros.
+       apply H;trivial. constructor. trivial. 
+       assert (HH:= intra _ _ _ H);simpl in HH.
+       apply HH;trivial. apply fixp;trivial.
+       generalize H;clear H;case r.
+       intros s'' Hcall r' Hint HP.
+       eapply Hc;eauto.
+       intros r' Hcall;eapply Hcr;eauto.
+     Qed.
+
+  Lemma JVM_IntraStepStar_ind : 
+    forall (p:JVM_Program) 
+     (P : JVM_Method -> JVM_IntraNormalState -> JVM_IntraNormalState + JVM_ReturnState -> Prop),
+       (forall m s, P m s (inl _ s)) ->
+       (forall m tau s r, JVM_exec_return p m tau s r -> P m s (inr _ r)) ->
+       (forall m tau s s' , JVM_exec_intra p m tau s s' -> 
+          forall r, JVM_IntraStepStar p m s' r -> P m s' r ->
+          P m s r) ->
+       (forall m tau s s' ret m' r, 
+          JVM_exec_call p m tau s ret m' s' (inr _ r) ->
+          JVM_IntraStepStar p m' s' (inr _ ret) ->
+          P m' s' (inr _ ret) ->
+          P m s (inr _ r)) ->
+       (forall m tau s s' ret m' s'' r, 
+          JVM_exec_call p m tau s ret m' s' (inl _ s'') ->
+          JVM_IntraStepStar p m' s' (inr _ ret) -> P m' s' (inr _ ret) ->
+          JVM_IntraStepStar p m s'' r -> P m s'' r ->
+          P m s r) ->
+    forall m s r, JVM_IntraStepStar p m s r -> P m s r.
+   Proof.
+     intros p Q H0 Hr Hi Hcr Hc.
+     fix fixp 4;intros m s' s Ht;case Ht;clear Ht s' s;intros.
+     apply H0.
+     generalize (JVM_IntraStep_ind_ Q H0 Hr Hi Hcr Hc H).
+     case r;intros;trivial.
+     apply H1;trivial. 
+     constructor.
+     assert (HH:=JVM_IntraStep_ind_ Q H0 Hr Hi Hcr Hc H);simpl in HH.
+     apply HH;trivial.   
+     apply fixp;trivial.
+   Qed.
+
+End JVM_instr.
+ 
+End JVM_BigStepAnnot.
