JVM_step.v
@@ -1,0 +1,567 @@
+(** Static Intra-method control flow step. We also implement an iterator on it *)
+
+Require Export Annotated.
+Import JVM_StaticHandler.JVM_StaticHandler JVM_BigStep.JVM_Dom JVM_Prog.
+
+
+  Section JVM_S_section.   (** step relation **)
+    Variable p : JVM_Program.
+    Variable subclass_test : JVM_ClassName -> JVM_ClassName -> bool.
+    Variable m : JVM_Method.
+
+    (* DEX Definition handler := handler subclass_test m. *)
+
+    Inductive JVM_step : JVM_PC -> JVM_Instruction -> JVM_tag -> option JVM_PC -> Prop :=
+    | aconst_null : forall i j,
+      next m i = Some j ->
+      JVM_step i Aconst_null None (Some j)
+    | arraylength : forall i j,
+      next m i = Some j ->
+      JVM_step i Arraylength None (Some j)
+(* DEX    
+    | arraylength_np_caught : forall i t,
+      In np (throwableAt m i) ->
+      handler i np = Some t ->
+      step i Arraylength (Some np) (Some t)
+    | arraylength_np_uncaught : forall i,
+      In np (throwableAt m i) ->
+      handler i np = None ->
+      step i Arraylength (Some np) None
+    | athrow_caught : forall e i t,
+      In e (throwableAt m i) ->
+      handler i e = Some t ->
+      step i Athrow (Some e) (Some t)
+    | athrow_uncaught : forall e i,
+      In e (throwableAt m i) ->
+      handler i e = None ->
+      step i Athrow (Some e) None
+*)
+(* DEX
+    | checkcast1 : forall i t j,
+      next m i = Some j ->
+      step i (Checkcast t) None (Some j)
+*)
+(* DEX
+    | checkcast_caught : forall i t te,
+      In cc (throwableAt m i) ->
+      handler i cc = Some te ->
+      step i (Checkcast t) (Some cc) (Some te)
+    | checkcast_uncaught : forall i t,
+      In cc (throwableAt m i) ->
+      handler i cc = None ->
+      step i (Checkcast t) (Some cc) None
+*)
+    | const : forall i t z j,
+      next m i = Some j ->
+      JVM_step i (Const t z) None (Some j)
+    | dup : forall i j,
+      next m i = Some j ->
+      JVM_step i Dup None (Some j)
+    | dup_x1 : forall i j,
+      next m i = Some j ->
+      JVM_step i Dup_x1 None (Some j)
+    | dup_x2 : forall i j,
+      next m i = Some j ->
+      JVM_step i Dup_x2 None (Some j)
+    | dup2 : forall i j,
+      next m i = Some j ->
+      JVM_step i Dup2 None (Some j)
+    | dup2_x1 : forall i j,
+      next m i = Some j ->
+      JVM_step i Dup2_x1 None (Some j)
+    | dup2_x2 : forall i j,
+      next m i = Some j ->
+      JVM_step i Dup2_x2 None (Some j)
+    | getfield : forall i f j,
+      next m i = Some j ->
+      JVM_step i (Getfield f) None (Some j)
+(* DEX
+    | getfield_np_caught : forall i t f,
+      In np (throwableAt m i) ->
+      handler i np = Some t ->
+      step i (Getfield f) (Some np) (Some t)
+    | getfield_np_uncaught : forall i f,
+      In np (throwableAt m i) ->
+      handler i np = None ->
+      step i (Getfield f) (Some np) None
+*)
+    | goto : forall i o,
+      JVM_step i (Goto o) None (Some (JVM_OFFSET.jump i o))
+    | i2b : forall i j,
+      next m i = Some j ->
+      JVM_step i I2b None (Some j)
+    | i2s : forall i j,
+      next m i = Some j ->
+      JVM_step i I2s None (Some j)
+    | ibinop : forall i op j,
+      next m i = Some j ->
+      JVM_step i (Ibinop op) None (Some j)
+(* DEX
+    | ibinop_ae_caught : forall i t op,
+      In ae (throwableAt m i) ->
+      op = DivInt \/ op = RemInt ->
+      handler i ae = Some t ->
+      step i (Ibinop op) (Some ae) (Some t)
+    | ibinop_ae_uncaught : forall i op,
+      In ae (throwableAt m i) ->
+      op = DivInt \/ op = RemInt ->
+      handler i ae = None ->
+      step i (Ibinop op) (Some ae) None
+*)
+    | if_acmp : forall i cmp o j,
+      next m i = Some j \/ j = JVM_OFFSET.jump i o ->
+      JVM_step i (If_acmp cmp o) None (Some j)
+    | if_icmp : forall i cmp o j,
+      next m i = Some j \/ j = JVM_OFFSET.jump i o ->
+      JVM_step i (If_icmp cmp o) None (Some j)
+    | ifeq : forall i cmp o j,
+      next m i = Some j \/ j = JVM_OFFSET.jump i o ->
+      JVM_step i (If0 cmp o) None (Some j)
+    | ifnull : forall i cmp o j,
+      next m i = Some j \/ j = JVM_OFFSET.jump i o ->
+      JVM_step i (Ifnull cmp o) None (Some j)
+    | iinc : forall i x c j,
+      next m i = Some j ->
+      JVM_step i (Iinc x c) None (Some j)
+    | ineg : forall i j,
+      next m i = Some j ->
+      JVM_step i Ineg None (Some j)
+    | instanceof : forall i t j,
+      next m i = Some j ->
+      JVM_step i (Instanceof t) None (Some j)
+    | invokestatic : forall i mid j,
+      next m i = Some j ->
+      JVM_step i (Invokestatic mid) None (Some j)
+(* DEX
+    | invokestatic_caught : forall i mid t e,
+      In e (throwableBy p (snd mid)) -> 
+      handler i e = Some t ->
+      step i (Invokestatic mid) (Some e) (Some t)
+    | invokestatic_uncaught : forall i mid e,
+      In e (throwableBy p (snd mid)) -> 
+      handler i e = None ->
+      step i (Invokestatic mid) (Some e) None
+*)
+    | invokevirtual : forall i mid j,
+      next m i = Some j ->
+      JVM_step i (Invokevirtual mid) None (Some j)
+(* DEX
+    | invokevirtual_caught : forall i mid t e,
+      In e ((throwableAt m i)++throwableBy p (snd mid)) -> 
+      handler i e = Some t ->
+      step i (Invokevirtual mid) (Some e) (Some t)
+    | invokevirtual_uncaught : forall i mid e,
+      In e ((throwableAt m i)++throwableBy p (snd mid)) -> 
+      handler i e = None ->
+      step i (Invokevirtual mid) (Some e) None
+*)
+    | lookupswitch : forall i d l o,
+      In o (d::@map _ _ (@snd _ _) l) ->
+      JVM_step i (Lookupswitch d l) None (Some (JVM_OFFSET.jump i o))
+    | new : forall i c j,
+      next m i = Some j ->
+      JVM_step i (New c) None (Some j)
+    | newarray : forall i t j,
+      next m i = Some j ->
+      JVM_step i (Newarray t) None (Some j)
+(* DEX
+    | newarray_nase_caught : forall i t te,
+      In nase (throwableAt m i) ->
+      handler i nase = Some te ->
+      step i (Newarray t) (Some nase) (Some te)
+    | newarray_nase_uncaught : forall i t,
+      In nase (throwableAt m i) ->
+      handler i nase = None ->
+      step i (Newarray t) (Some nase) None
+*)
+    | nop : forall i j,
+      next m i = Some j ->
+      JVM_step i Nop None (Some j)
+    | pop : forall i j,
+      next m i = Some j ->
+      JVM_step i Pop None (Some j)
+    | pop2 : forall i j,
+      next m i = Some j ->
+      JVM_step i Pop2 None (Some j)
+    | putfield : forall i f j,
+      next m i = Some j ->
+      JVM_step i (Putfield f) None (Some j)
+(* DEX
+    | putfield_np_caught : forall i t f,
+      In np (throwableAt m i) ->
+      handler i np = Some t ->
+      step i (Putfield f) (Some np) (Some t)
+    | putfield_np_uncaught : forall i f,
+      In np (throwableAt m i) ->
+      handler i np = None ->
+      step i (Putfield f) (Some np) None
+*)
+    | return_ : forall i,
+      JVM_step i Return None None
+    | swap : forall i j,
+      next m i = Some j ->
+      JVM_step i Swap None (Some j)
+    | tableswitch : forall i d lo hi l o,
+      In o (d::l) ->
+      JVM_step i (Tableswitch d lo hi l) None (Some (JVM_OFFSET.jump i o))
+    | vaload : forall i t j,
+      next m i = Some j ->
+      JVM_step i (Vaload t)  None (Some j)
+(* DEX
+    | vaload_np_caught : forall i t te,
+      In np (throwableAt m i) ->
+      handler i np = Some te ->
+      step i (Vaload t) (Some np) (Some te)
+    | vaload_np_uncaught : forall i t,
+      In np (throwableAt m i) ->
+      handler i np = None ->
+      step i (Vaload t) (Some np) None
+    | vaload_iob_caught : forall i te t,
+      In iob (throwableAt m i) ->
+      handler i iob = Some te ->
+      step i (Vaload t) (Some iob) (Some te)
+    | vaload_iob_uncaught : forall i t,
+      In iob (throwableAt m i) ->
+      handler i iob = None ->
+      step i (Vaload t) (Some iob) None
+*)
+    | vastore : forall i t j,
+      next m i = Some j ->
+      JVM_step i (Vastore t) None (Some j)
+(* DEX
+    | vastore_np_caught : forall i t te,
+      In np (throwableAt m i) ->
+      handler i np = Some te ->
+      step i (Vastore t) (Some np) (Some te)
+    | vastore_np_uncaught : forall i t,
+      In np (throwableAt m i) ->
+      handler i np = None ->
+      step i (Vastore t) (Some np) None
+    | vastore_ase_caught : forall i t te,
+      In ase (throwableAt m i) ->
+      handler i ase = Some te ->
+      step i (Vastore t) (Some ase) (Some te)
+    | vastore_ase_uncaught : forall i t,
+      In ase (throwableAt m i) ->
+      handler i ase = None ->
+      step i (Vastore t) (Some ase) None
+    | vastore_iob_caught : forall i t te,
+      In iob (throwableAt m i) ->
+      handler i iob = Some te ->
+      step i (Vastore t) (Some iob) (Some te)
+    | vastore_iob_uncaught : forall i t,
+      In iob (throwableAt m i) ->
+      handler i iob = None ->
+      step i (Vastore t) (Some iob) None
+*)
+    | vload : forall i t x j,
+      next m i = Some j ->
+      JVM_step i (Vload t x) None (Some j)
+    | vstore : forall i t x j,
+      next m i = Some j ->
+      JVM_step i (Vstore t x) None (Some j)
+    | vreturn : forall i x,
+      JVM_step i (Vreturn x) None None.
+
+    Definition get_steps (i:JVM_PC) (ins:JVM_Instruction) (next:option JVM_PC): list (JVM_tag * option JVM_PC) := 
+      match ins with
+        | Arraylength => (None,next)::nil (* DEX ::(map (fun e => (Some e,handler i e)) (throwableAt m i)) *)
+        (* DEX | Athrow => map (fun e => (Some e,handler i e)) (throwableAt m i) *)
+        (* DEX | Checkcast _ => (None,next)::(Some cc,handler i cc)::nil *)
+        | Getfield _ => (None,next)::nil(* DEX ::(map (fun e => (Some e,handler i e)) (throwableAt m i)) *)
+        | Ibinop op => (None,next)::nil(* DEX ::
+          (match op with
+             | DivInt =>map (fun e => (Some e,handler i e)) (throwableAt m i)
+             | RemInt => map (fun e => (Some e,handler i e)) (throwableAt m i)
+             | _ => nil
+           end) *)
+        | Invokestatic mid => 
+          (None,next)::nil (* DEX ::(map (fun e => (Some e,handler i e)) ((throwableAt m i)++throwableBy p (snd mid))) *)
+        | Invokevirtual mid =>
+          (None,next)::nil (* DEX ::(map (fun e => (Some e,handler i e)) ((throwableAt m i)++throwableBy p (snd mid))) *)
+        | Lookupswitch d l =>
+          map (fun o => (None,Some (JVM_OFFSET.jump i o))) (d::@map _ _ (@snd _ _) l)
+        | Newarray _ =>  (None,next)::nil (* DEX ::(map (fun e => (Some e,handler i e)) (throwableAt m i)) *)
+        | Putfield _ => (None,next)::nil (* DEX ::(map (fun e => (Some e,handler i e)) (throwableAt m i)) *)
+        | Return => (None,None)::nil
+        | Tableswitch d lo hi l =>
+          map (fun o => (None,Some (JVM_OFFSET.jump i o))) (d::l) 
+        | Vaload _ => (None,next)::nil (* ::(map (fun e => (Some e,handler i e)) (throwableAt m i)) *)
+        | Vastore _ => (None,next)::nil (*::(map (fun e => (Some e,handler i e)) (throwableAt m i)) *)
+        | Vreturn _ => (None,None)::nil
+        | Goto o => (None,Some (JVM_OFFSET.jump i o))::nil
+        | If_acmp cmp o => (None,next)::(None,Some (JVM_OFFSET.jump i o))::nil
+        | If_icmp cmp o => (None,next)::(None,Some (JVM_OFFSET.jump i o))::nil
+        | If0 cmp o => (None,next)::(None,Some (JVM_OFFSET.jump i o))::nil
+        | Ifnull cmp o => (None,next)::(None,Some (JVM_OFFSET.jump i o))::nil
+        | _ => (None,next)::nil
+      end.
+
+    Lemma all_step_in_get_steps : forall i ins tau oj,
+        JVM_step i ins tau oj -> 
+        In (tau,oj) (get_steps i ins (next m i)).
+    Proof.
+      intros.
+      inversion_clear H; simpl get_steps; try rewrite H0; auto with datatypes;
+      (* DEX try match goal with
+        [ id : handler _ _ = ?x |- _ ] => 
+        pattern x at 1; rewrite <- id
+          end; *)
+      try (
+        repeat ((left; reflexivity)||right);
+          try match goal with
+                [ |- In (_,_) (map ?F _) ] => 
+                apply in_map with (f:=F); try assumption;
+                  apply in_or_app; auto
+              end; fail).
+(* DEX
+      right;
+      try match goal with
+      [ |- In (_,_) (map ?F _) ] => 
+      apply in_map with (f:=F); try assumption
+      end.
+      destruct H0; subst; simpl; auto with datatypes;
+      try match goal with
+      [ |- In (_,_) (map ?F _) ] => 
+            apply in_map with (f:=F); try assumption
+      end.
+      right; destruct H; subst; simpl; auto with datatypes;
+      try match goal with
+      [ |- In (_,_) (map ?F _) ] => 
+            apply in_map with (f:=F); try assumption
+      end.
+*)
+      destruct H0 as [H0|H0]; rewrite <- H0; auto with datatypes.
+      destruct H0 as [H0|H0]; rewrite <- H0; auto with datatypes.
+      destruct H0 as [H0|H0]; rewrite <- H0; auto with datatypes.
+      destruct H0 as [H0|H0]; rewrite <- H0; auto with datatypes.
+      destruct H0; subst.
+      left; reflexivity.
+      right; match goal with
+      [ |- In (_,_) (map ?F _) ] => 
+      apply in_map with (f:=F); try assumption
+      end.
+      destruct H0; subst.
+      left; reflexivity.
+      right; match goal with
+      [ |- In (_,_) (map ?F _) ] => 
+      apply in_map with (f:=F); try assumption
+      end.
+    Qed.
+
+  Section for_all_steps.
+    Variable test : JVM_PC -> JVM_Instruction -> JVM_tag -> option JVM_PC -> bool.
+
+    Definition for_all_steps_bm (bm:JVM_BytecodeMethod) : bool :=
+      MapN.for_all _
+      (fun i (ins_next:JVM_Instruction*(option JVM_PC*list JVM_ClassName)) =>
+        let (ins,next) := ins_next in
+          for_all _
+          (fun (tau_oj:JVM_tag*option JVM_PC) => let (tau,oj):=tau_oj in test i ins tau oj)
+          (get_steps i ins (fst next)))
+      bm.(JVM_BYTECODEMETHOD.instr).
+
+    Lemma for_all_steps_bm_true : forall bm,
+      JVM_METHOD.body m = Some bm ->
+      for_all_steps_bm bm = true ->
+      forall i ins tau oj,
+        instructionAt m i = Some ins ->
+        JVM_step i ins tau oj -> test i ins tau oj = true.
+    Proof.
+      intros.
+      assert (T1:=MapN.for_all_true _ _ _ H0).
+      assert (T2:=all_step_in_get_steps _ _ _ _ H2).
+      unfold instructionAt, JVM_BYTECODEMETHOD.instructionAt in H1.
+      rewrite H in H1.
+      caseeq (MapN.get (JVM_Instruction * (option JVM_PC*list JVM_ClassName)) (JVM_BYTECODEMETHOD.instr bm) i).
+      intros (ins0,next0) T3.
+      rewrite T3 in H1.
+      generalize (T1 _ _ T3); clear T1; intros T1.
+      apply for_all_true with
+        (test:=(fun tau_oj : JVM_tag * option JVM_PC =>
+          let (tau, oj) := tau_oj in test i ins tau oj))
+        (2:=T2).
+      unfold next, JVM_BYTECODEMETHOD.nextAddress.
+      rewrite H; rewrite T3; simpl.
+      inversion_mine H1; auto.
+      intros T3; rewrite T3 in H1; discriminate.
+    Qed.
+
+  Definition for_all_steps_m : bool :=
+    match JVM_METHOD.body m with
+      | None => false
+      | Some bm => for_all_steps_bm bm
+    end.
+
+  Definition test_all_steps_m : list (JVM_PC*bool) :=
+    match JVM_METHOD.body m with
+      | None => nil
+      | Some bm => 
+      List.map
+      (fun (ins_next:JVM_PC*(JVM_Instruction*(option JVM_PC*list JVM_ClassName))) =>
+        let (i,ins_next) := ins_next in
+        let (ins,next) := ins_next in
+          (i,for_all _
+            (fun (tau_oj:JVM_tag*option JVM_PC) => let (tau,oj):=tau_oj in test i ins tau oj)
+            (get_steps i ins (fst next))))
+      (MapN.elements _ bm.(JVM_BYTECODEMETHOD.instr))
+    end.
+
+  Lemma for_all_steps_m_true : for_all_steps_m = true ->
+      forall i ins tau oj,
+        instructionAt m i = Some ins ->
+        JVM_step i ins tau oj -> test i ins tau oj = true.
+  Proof.
+    unfold for_all_steps_m.
+    generalize for_all_steps_bm_true.
+    destruct (JVM_METHOD.body m) as [bm|]; intro.
+    apply H; auto.
+    intros; discriminate.
+  Qed.
+
+  End for_all_steps.
+
+  Section for_all_succs.
+    Variable pc:JVM_PC.
+    Variable test : JVM_tag -> option JVM_PC -> bool.
+
+    Definition for_all_succs_bm (bm:JVM_BytecodeMethod) : bool :=
+      match MapN.get _ bm.(JVM_BYTECODEMETHOD.instr) pc with
+        | None => true
+        | Some (ins,(op,l)) => 
+          for_all _
+          (fun (tau_oj:JVM_tag*option JVM_PC) => let (tau,oj):=tau_oj in test tau oj)
+          (get_steps pc ins op)
+      end.
+
+    Lemma for_all_succs_bm_true : forall bm,
+      JVM_METHOD.body m = Some bm ->
+      for_all_succs_bm bm = true ->
+      forall ins tau oj,
+        instructionAt m pc = Some ins ->
+        JVM_step pc ins tau oj -> test tau oj = true.
+    Proof.
+      unfold for_all_succs_bm; intros.
+      assert (T2:=all_step_in_get_steps _ _ _ _ H2).
+      unfold instructionAt, JVM_BYTECODEMETHOD.instructionAt in H1.
+      rewrite H in H1.
+      caseeq (MapN.get (JVM_Instruction * (option JVM_PC*list JVM_ClassName)) (JVM_BYTECODEMETHOD.instr bm) pc).
+      intros (ins0,next0) T3.
+      rewrite T3 in H1; rewrite T3 in H0.
+      destruct next0.
+      apply for_all_true with
+        (test:=(fun tau_oj : JVM_tag * option JVM_PC =>
+          let (tau, oj) := tau_oj in test tau oj))
+        (2:=T2).
+      unfold next, JVM_BYTECODEMETHOD.nextAddress.
+      inversion_mine H1.
+      rewrite H; rewrite T3; simpl; auto.
+      intros.
+      rewrite H3 in H1; discriminate.
+    Qed.
+
+  Definition for_all_succs_m : bool :=
+    match JVM_METHOD.body m with
+      | None => false
+      | Some bm => for_all_succs_bm bm
+    end.
+
+  Lemma for_all_succs_m_true : for_all_succs_m = true ->
+      forall ins tau oj,
+        instructionAt m pc = Some ins ->
+        JVM_step pc ins tau oj -> test tau oj = true.
+  Proof.
+    unfold for_all_succs_m.
+    generalize for_all_succs_bm_true.
+    destruct (JVM_METHOD.body m) as [bm|]; intro.
+    apply H; auto.
+    intros; discriminate.
+  Qed.
+   
+ End for_all_succs.
+
+  Section for_all_instrs.
+    Variable test : JVM_PC -> JVM_Instruction -> bool.
+
+    Definition for_all_instrs_bm (bm:JVM_BytecodeMethod) : bool :=
+      MapN.for_all _
+      (fun i (ins_next:JVM_Instruction*(option JVM_PC*list JVM_ClassName)) =>
+        let (ins,next) := ins_next in test i ins)
+      bm.(JVM_BYTECODEMETHOD.instr).
+
+    Lemma for_all_instrs_bm_true : forall bm,
+      JVM_METHOD.body m = Some bm ->
+      for_all_instrs_bm bm = true ->
+      forall i ins,
+        instructionAt m i = Some ins -> test i ins = true.
+    Proof.
+      intros.
+      assert (T1:=MapN.for_all_true _ _ _ H0).
+      unfold instructionAt, JVM_BYTECODEMETHOD.instructionAt in H1.
+      rewrite H in H1.
+      caseeq (MapN.get (JVM_Instruction * (option JVM_PC*list JVM_ClassName)) (JVM_BYTECODEMETHOD.instr bm) i).
+      intros (ins0,next0) T3.
+      rewrite T3 in H1.
+      generalize (T1 _ _ T3); clear T1; intros T1.
+      inversion_mine H1; auto.
+      intros T3; rewrite T3 in H1; discriminate.
+    Qed.
+
+    Definition for_all_instrs_m : bool :=
+      match JVM_METHOD.body m with
+        | None => false
+        | Some bm => for_all_instrs_bm bm
+      end.
+
+    Lemma for_all_instrs_m_true : for_all_instrs_m = true ->
+      forall i ins,
+        instructionAt m i = Some ins -> test i ins = true.
+    Proof.
+      unfold for_all_instrs_m.
+      generalize for_all_instrs_bm_true.
+      destruct (JVM_METHOD.body m) as [bm|]; intro.
+      apply H; auto.
+      intros; discriminate.
+    Qed.
+
+  End for_all_instrs.
+
+End JVM_S_section.
+
+Module JVM_MapClassTools := MapProjTools JVM_PROG.JVM_MapClass.
+
+Section p.
+  Variable p : JVM_Program.
+
+  Definition ValidMethod (m:JVM_Method) : Prop :=
+    exists c, JVM_PROG.defined_Class p c /\ JVM_CLASS.defined_Method c m.
+
+  Variable test : JVM_Method -> bool.
+
+  Definition for_all_methods : bool :=
+    JVM_MapClassTools.for_all
+    (fun cl =>  JVM_MapShortMethSign.for_all _ (fun _ => test) cl.(JVM_CLASS.methods))
+    p.(JVM_PROG.classes_map).
+
+  Lemma for_all_methods_true : for_all_methods = true ->
+    forall m, ValidMethod m -> test m = true.
+  Proof.
+    intros.
+    destruct H0 as [c [H0 H1]].
+    generalize (JVM_MapClassTools.for_all_true _ _ H _ H0); intros.
+    unfold JVM_CLASS.defined_Method, JVM_CLASS.method in H1.
+    caseeq (JVM_MapShortMethSign.get JVM_Method (JVM_CLASS.methods c) (JVM_METHOD.signature m)); intros.
+    rewrite H3 in H1.
+    destruct (JVM_METHODSIGNATURE.eq_t (JVM_METHOD.signature m) (JVM_METHOD.signature j)); inversion_mine H1.
+    apply (JVM_MapShortMethSign.for_all_true _ _ _ H2 _ _ H3).
+    rewrite H3 in H1; discriminate.
+  Qed.
+
+End p.
+
+
+  
+
+
+
+
