LoadBicolano.v
@@ -1,10 +1,7 @@
 (** * Entry point in Bicolano semantics *)
 
 Require Export Tactics.
-Require Export StaticHandler.
-Require Export ImplemDomain.
-
-
-
-
-
+Require Export DEX_StaticHandler.
+Require Export JVM_StaticHandler.
+Require Export DEX_ImplemDomain.
+Require Export JVM_ImplemDomain.
